

# CSE 317: Design and Analysis of Algorithms

---

Shahid Hussain

Recurrences: Fall 2024

# Recurrences

---

# Recurrences

- Recurrences (or recurrence relations or difference equations) arise naturally during analysis of algorithms
- For example, most recursive algorithms can be represented by a recurrence and then the time complexity of the algorithm is just the solution of the recurrence
- For example consider the following recursive algorithm that computes  $n!$  for any  $n \geq 1$

**Algorithm:** FACTORIAL

**Input:** An integer  $n \geq 1$

**Output:** The value of  $n!$

1. **if**  $n = 1$  **then return** 1
2. **else return**  $n * \text{FACTORIAL}(n - 1)$

# Recurrences

- Assume that the time to compute factorial of an integer  $n \geq 1$  is represented as  $T(n)$
- Clearly  $T(n) = 1 + T(n - 1)$ , furthermore,  $T(1) = 1$
- We can solve this recurrence as following:

$$\begin{aligned}T(n) &= 1 + T(n - 1) \\&= 1 + 1 + T(n - 2) \\&= 1 + 1 + 1 + T(n - 3) \\&\quad \dots \\&= 1 + 1 + 1 + \dots + 1 + T(1) \\&= n = \Theta(n)\end{aligned}$$

# A Simple Recurrence

- Consider the following recurrence:

$$A(n) = 2A(n-1) + 1, \quad \text{such that } A(0) = 0$$

- First few terms of the sequence are: 0, 1, 3, 7, 15, 31, 63, ...
- It seems like  $A(n) = 2^n - 1$
- We can prove this by induction
- Base case:  $A(0) = 0 = 2^0 - 1$
- Inductive step: Assume that  $A(k) = 2^k - 1$  for all  $k < n$
- Then for  $n = k + 1$  we have:

$$A(k+1) = 2A(k) + 1 = 2(2^k - 1) + 1 = 2^{k+1} - 2 + 1 = 2^{k+1} - 1$$

## A Simple Recurrence

- We can also solve this recurrence by expanding the recursive term as follows:

$$\begin{aligned}A(n) &= 2A(n-1) + 1 \\&= 2(2A(n-2) + 1) + 1 \\&= 2^2A(n-2) + 2 + 1 \\&= 2^2(2A(n-3) + 1) + 2 + 1 \\&= 2^3A(n-3) + 2^2 + 2 + 1 \\&\quad \dots \\&= 2^n A(0) + 2^{n-1} + 2^{n-2} + \dots + 2^2 + 2 + 1 \\&= 2^n - 1 = \Theta(2^n)\end{aligned}$$

# A General Two Terms Recurrence

## One Term Recurrence with Constant Coefficient

A recurrence of the following form, where  $a$  and  $c > 0$  are constants and  $f(n)$  is a function of  $n$ :

$$A(n) = cA(n-1) + f(n), \quad \text{such that} \quad A(0) = a$$

has the solution:

$$A(n) = a \cdot c^n + \sum_{j=0}^{n-1} c^j \cdot f(n-j).$$

# Proof for Two Terms Recurrences

$$\begin{aligned}A(n) &= cA(n-1) + f(n) \\&= c(cA(n-2) + f(n-1)) + f(n) \\&= c^2A(n-2) + cf(n-1) + f(n) \\&= c^2(cA(n-3) + f(n-2)) + cf(n-1) + f(n) \\&= c^3A(n-3) + c^2f(n-2) + cf(n-1) + f(n) \\&\quad \dots \\&= c^n A(0) + c^{n-1}f(1) + c^{n-2}f(2) + \dots + cf(n-1) + f(n) \\&= a \cdot c^n + \sum_{j=0}^{n-1} c^j \cdot f(n-j).\end{aligned}$$



# Linear Homogeneous Recurrences

- A *linear homogeneous recurrence of degree  $k$*  with constant Coefficients is a recurrence relation which has  $k$  recursive terms and is of the form:

$$A(n) = c_1A(n-1) + c_2A(n-2) + \cdots + c_kA(n-k)$$

where  $c_i$ 's are constants and  $c_k \neq 0$  with  $A(0) = C_0, \dots, A(k-1) = C_{k-1}$  as  *$k$  initial conditions*

- We can solve this recurrence by finding the roots of the corresponding characteristic equation

# Linear Homogeneous Recurrences

- We can rewrite the recurrence as follows:

$$A(n) - c_1A(n-1) - c_2A(n-2) - \cdots - c_kA(n-k) = 0$$

- The corresponding characteristic equation is:

$$x^k - c_1x^{k-1} - c_2x^{k-2} - \cdots - c_k = 0$$

- The roots of this equation  $r_1, r_2, \dots, r_k$  will be used to form the general solution of the recurrence
- The general solution of the recurrence is:

$$A(n) = \alpha_1 r_1^n + \alpha_2 r_2^n + \cdots + \alpha_k r_k^n$$

# The Fibonacci Recurrence

- Let  $f_n = f_{n-1} + f_{n-2}$  with  $f_0 = 0$  and  $f_1 = 1$  ( $n \geq 0$ )
- We can rewrite it as:  $f_n - f_{n-1} - f_{n-2} = 0$
- The characteristic equation is:  $x^2 - x - 1 = 0$
- The two real roots of this equation are:  $\frac{1 \pm \sqrt{5}}{2}$
- Thus the general solution of the Fibonacci recurrence is:

$$f_n = \alpha_1 \left( \frac{1 + \sqrt{5}}{2} \right)^n + \alpha_2 \left( \frac{1 - \sqrt{5}}{2} \right)^n$$

- We can find the exact values of  $\alpha_1$  and  $\alpha_2$  by using the initial conditions,  $\alpha_1 = \frac{1}{\sqrt{5}}$  and  $\alpha_2 = -\frac{1}{\sqrt{5}}$

## Another Three Term Recurrence

- Consider the recurrence:  $a_n = a_{n-1} - a_{n-2}$  with  $a_0 = 0$  and  $a_1 = 1$  ( $n \geq 2$ )
- The first few terms of the sequence are:  
 $0, 1, 1, 0, -1, -1, 0, \dots$
- The characteristic equation is:  $x^2 - x + 1 = 0$  which has the roots:  $\frac{1}{2} \pm i\frac{\sqrt{3}}{2}$ ,
- These roots can be written in polar coordinates as:

$$x_1 = re^{-i\theta} \quad \text{and} \quad x_2 = re^{i\theta}$$

- Here  $r = \sqrt{(1/2)^2 + (\sqrt{3}/2)^2} = 1$  and  $\theta = \tan^{-1} \sqrt{3} = \pi/3$

## Another Three Term Recurrence

- Let us find  $x_1^n$  and  $x_2^n$ :

$$\begin{aligned}x_1^n &= (re^{-i\theta})^n = r^n e^{-in\theta} = e^{-i\pi n/3} \\&= \cos\left(\frac{-\pi n}{3}\right) + i \sin\left(\frac{-\pi n}{3}\right) \\&= \cos\left(\frac{\pi n}{3}\right) - i \sin\left(\frac{\pi n}{3}\right) \\x_2^n &= (re^{i\theta})^n = r^n e^{in\theta} = e^{i\pi n/3} \\&= \cos\left(\frac{\pi n}{3}\right) + i \sin\left(\frac{\pi n}{3}\right)\end{aligned}$$

- We can thus find the general solution as

$$\begin{aligned}a_n &= \alpha_1 x_1^n + \alpha_2 x_2^n \\&= \alpha_1 \left[ \cos\left(\frac{\pi n}{3}\right) - i \sin\left(\frac{\pi n}{3}\right) \right] \\&\quad + \alpha_2 \left[ \cos\left(\frac{\pi n}{3}\right) + i \sin\left(\frac{\pi n}{3}\right) \right]\end{aligned}$$

## Another Three Term Recurrence

- We know that  $a_0 = 0$  therefore:

$$0 = \alpha_1 [\cos 0 - i \sin 0] + \alpha_2 [\cos 0 + i \sin 0]$$

$$0 = \alpha_1 + \alpha_2 \implies \alpha_1 = -\alpha_2$$

- Similarly, we know that  $a_1 = 1$  therefore:

$$1 = \alpha_1 \left[ \cos \left( \frac{\pi}{3} \right) - i \sin \left( \frac{\pi}{3} \right) \right]$$

$$+ \alpha_2 \left[ \cos \left( \frac{\pi}{3} \right) + i \sin \left( \frac{\pi}{3} \right) \right]$$

$$= \alpha_1 \left[ \cos \left( \frac{\pi}{3} \right) - i \sin \left( \frac{\pi}{3} \right) \right]$$

$$- \alpha_1 \left[ \cos \left( \frac{\pi}{3} \right) + i \sin \left( \frac{\pi}{3} \right) \right]$$

$$1 = -2i\alpha_1 \sin \left( \frac{\pi}{3} \right) = -2i\alpha_1 \frac{\sqrt{3}}{2} \implies$$

$$\alpha_1 = -\frac{1}{i\sqrt{3}} \quad \text{and} \quad \alpha_2 = \frac{1}{i\sqrt{3}}$$

## Another Three Term Recurrence

- Therefore the general solution of the recurrence is:

$$\begin{aligned}a_n &= \frac{1}{i\sqrt{3}} \left[ \cos\left(\frac{\pi n}{3}\right) + i \sin\left(\frac{\pi n}{3}\right) \right] \\&\quad - \frac{1}{i\sqrt{3}} \left[ \cos\left(\frac{\pi n}{3}\right) - i \sin\left(\frac{\pi n}{3}\right) \right] \\a_n &= \frac{2}{\sqrt{3}} \sin\left(\frac{\pi n}{3}\right)\end{aligned}$$